\documentclass{article}
\usepackage{amsmath}
\usepackage{algorithm}
\usepackage{algorithmic}
\usepackage{graphicx}
\usepackage{program}
\usepackage{mathtools}
\usepackage{float}
\usepackage{fancyvrb}
\usepackage{amsfonts}
\newcommand{\overbar}[1]{\mkern 1.5mu\overline{\mkern-1.5mu#1\mkern-1.5mu}\mkern 1.5mu}

\DeclarePairedDelimiter\floor{\lfloor}{\rfloor}
\begin{document}
	Given recursive definition
	\begin{equation}
		F_{2^t} = (\prod_{c=1}^{t}(I_{2^{c-1}}\otimes F_2 \otimes I_{2^{t-c}})(I_{2^{c-1}} \otimes T^{2^{t-c+1}}_{2^{t-c}}))R_{2^t}
	\end{equation}
	Where
	\begin{equation}
		T^{mn}_n(e^m_i \otimes e^n_j)=\omega^{ij}(e^m_i \otimes e^n_j)
	\end{equation}
	and 
	\begin{equation}
		L^{mn}_n(e^m_i \otimes e^n_j) = (e^n_j \otimes e^m_i)
	\end{equation}
	From this we can get
	\begin{equation}
		F_{2^t} = (\prod_{c=1}^{t}L_2^{2^t}(I_{2^{t-1}}\otimes F_2)T_c)R_{2^t}
	\end{equation}
	where 
	\begin{equation}
		T_c = L^{2^t}_{2^{t-c}}(I_{2^{c-1}} \otimes T^{2^{t-c+1}}_{2^{t-c}})L^{2^t}_{2^c}
	\end{equation}
	and
	\begin{equation}
		A^{m \times m} \otimes B^{n\times n}=L^{mn}_m(B^{n \times n} \otimes A^{m \times m})L^{mn}_n
	\end{equation}

	1.
	\begin{equation}
		T^{mn}_n(e^m_i \otimes e^n_j)=\omega^{ij}(e^m_i \otimes e^n_j)
	\end{equation}
	while
	\begin{equation}
		W_ne^n_i= \omega^ie^n_i
	\end{equation}
	
	So for $T^{mn}_n(e^m_i \otimes e^n_j)=\omega^{ij}(e^m_i \otimes e^n_j)$, if we have
	$T^{'mn}_n$ just be a diagonal of $W_n$s repeating we get
	\begin{equation}
		T^{'mn}_n(e^m_i \otimes e^n_j)=\omega^{i}(e^m_i \otimes e^n_j)
	\end{equation}
	Thus as 
	\begin{equation}
		(W_n)^je^n_i= \omega^{ij}e^n_i
	\end{equation}
	
	\begin{equation}
		T^{mn}_n(e^m_i \otimes e^n_j)=\omega^{ij}(e^m_i \otimes e^n_j)
	\end{equation}
	$T^{'mn}_n$ just be a diagonal of $W_n^j$ from j 0 to m. So
	
	\begin{equation}
		T^{mn}_n = \oplus_{i=0}^{m-1} W^i_n(\omega)
	\end{equation}
	
	2.
	\begin{align}
		L^{mn}_nT^{mn}_nL^{mn}_m(e^n_i \otimes e^m_j)&=L^{mn}_nT^{mn}_n(e^m_j \otimes e^n_i)\\
		&=\omega^{ij}L^{mn}_n(e^m_j \otimes e^n_i) \\
		&=\omega^{ij}(e^n_i \otimes e^{m}_j) \\
		&= T^{mn}_m(e^n_i \otimes e^{m}_j) 
	\end{align}	

	3. 
	With $m=2^c$, $n=2^{t-c}$
	\begin{align}
		T_c &= L^{2^t}_{2^{t-c}}(I_{2^{c-1}} \otimes T^{2^{t-c+1}_{2^{t-c}}}) L^{2^t}_{2^c} \\
		&=(L^{2^t}_{2^{t-c}}I_{2^{c-1}}L^{2^t}_{2^c} \otimes L^{2^t}_{2^{t-c}}T^{2^{t-c+1}_{2^{t-c}}}L^{2^t}_{2^c}) \\
		&= (I_{2^{c-1}} \otimes T^{2^{t-c+1}}_{2})
	\end{align}
	As
	\begin{equation}
		T^{mn}_n = \oplus_{i=0}^{m-1} W^i_n(\omega)
	\end{equation}
	\begin{align}
		&= I_{2^{c-1}} \otimes \oplus_{i=0}^{2^{t-c}-1} W^i_2(\omega)
	\end{align}
	how where did the $2^c$ come from?
	
	4.
	\begin{align}
		F_{2^t} &= (\prod_{c=1}^{t}(I_{2^{c-1}}\otimes F_2 \otimes I_{2^{t-c}})(I_{2^{c-1}} \otimes T^{2^{t-c+1}}_{2^{t-c}}))R_{2^t} \\
		&= (\prod_{c=1}^{t}L^{2^t}_{2^{c-1}}(F_2 \otimes I_{2^{t-c}} \otimes I_{2^{c-1}} )L^{2^t}_{2^{t-c+1}} L^{2^t}_{2^{c-1}}( T^{2^{t-c+1}}_{2^{t-c}}  \otimes I_{2^{c-1}})L^{2^t}_2L^{2^t}_{2^{t-c}})R_{2^t} \\
		&=(\prod_{c=1}^{t}L^{2^t}_{2^{c-1}}(F_2 \otimes I_{2^{t-1}} )( T^{2^{t-c+1}}_{2^{t-c}}  \otimes I_{2^{c-1}})L^{2^t}_{2^{t-c+1}})R_{2^t}
	\end{align}
	final step hmm
	\begin{align}
		(F_2 \otimes I_{2^t})T^{2^{t+1}}_{2^t}(F_{2^t} \otimes I_2)L^{2^{t+1}}_2
	\end{align}
	
	5.
	
	\begin{align}
		F_{2^t} &= (\prod_{c=1}^{t}L_2^{2^t}(I_{2^{t-1}}\otimes F_2)T_c)R_{2^t} \\
		&= (\prod_{c=1}^{t}L_2^{2^t}(I_{2^{t-1}}\otimes F_2)L^{2^t}_{2^{t-c}}(I_{2^{c-1}} \otimes T^{2^{t-c+1}_{2^{t-c}}}) L^{2^t}_{2^c})R_{2^t} \\
		&= (\prod_{c=1}^{t}L_2^{2^t}L_{2^{t-1}}^{2^t}(F_2 \otimes I_{2^{t-1}})L_2^{2^t}L^{2^t}_{2^{t-c}}L_{2^{c-1}}^{2^t}(T^{2^{t-c+1}}_{2^{t-c}} \otimes I_{2^{c-1}})L_{2^{t-c+1}}^{2^{t}}L^{2^t}_{2^c})R_{2^t} \\
		&= (\prod_{c=1}^{t}(F_2 \otimes I_{2^{t-1}})L_{2^{c}}^{2^t}(T^{2^{t-c+1}}_{2} \otimes I_{2^{c-1}})L_{2}^{2^{t}})R_{2^t} \\
	\end{align}

\end{document}